\سؤال{}

$$
\int_{-\infty}^{+\infty} N(\theta | 0, 1) d\theta = 1 \xRightarrow{Symmetric} 
\begin{cases}
\int_{-\infty}^{0}N(\theta | 0, 1)d\theta = \frac{1}{2} \\
\int_{0}^{\infty}N(\theta | 0, 1)d\theta = \frac{1}{2}
\end{cases}
$$

$$
\phi(a)  = \int_{-\infty}^{a} N(\theta | 0, 1) d\theta = \int_{-\infty}^{0} N(\theta | 0, 1) d\theta + \int_{0}^{a} N(\theta | 0, 1) d\theta =
 \frac{1}{2} + \int_{0}^{a} \frac{1}{2\pi} e^{\frac{-\theta^2}{2}d}\theta
$$
با اعمال تغییر متغیر و انتگرال‌گیری خواهیم داشت:
$$
\phi(a) = \frac{1}{2} + \frac{1}{2} \int_{0}^{\frac{a}{\sqrt{2}}} \frac{2}{\sqrt{\pi}}e^{-\theta^2}d\theta
= \frac{1}{2}(1 + \frac{2}{\sqrt{\pi}}\int_{0}^{\frac{a}{\sqrt{2}}}e^{-\theta^2}d\theta) \implies \phi(a) = \frac{1}{2}(1 + erf(\frac{a}{\sqrt{2}}))
$$