\سؤال{}


اگر $y_n = y(x_n, w)$ آن‌گاه داریم:
$$
y^{noisy}_n = w_0 + \Sigma_i^{D} w_i(x_{ni} + \epsilon_{ni}) 
= y_n + \Sigma_i^{D}w_i\epsilon_{ni}
$$

حال با استفاده از 
$
E_D(w) = \frac{1}{2} \Sigma_{n = 1}^{N}(y(x_n, w) - t_n)^2
$
داریم:
$$
E^{noisy} = 
\frac{1}{2}\Sigma_{n = 1}^{N}(y^{noisy}_{n} - t_n)^2 
= \frac{1}{2}\Sigma_{n =  1}^{N}(y_n^{noisy \: 2} - 2y_n^{noisy}t_n + t_n^2)
$$

$$
\rightarrow E^{noisy} = 
\frac{1}{2} \Sigma_{n = 1}^{N}(y_n^2 + 2y_n\Sigma_{i = 1}^{D}w_i\epsilon_{ni} + (\Sigma_{i = 1}^{D}w_i\epsilon_{ni})^2 - 2t_ny_n - 2t_n\Sigma_{i = 1}^{D}w_i\epsilon_{ni} + t_n^2)
$$

حال اگر امید ریاضی $E^{noisy}$را بگیریم که جملع‌ی  $2y_n\Sigma_{i = 1}^{D}w_i\epsilon_{ni}$ و جمله‌ی 
$
- 2t_n\Sigma_{i = 1}^{D}w_i\epsilon_{ni} + t_n^2
$
به دلیل 
$
\mathbb{E}(\epsilon_{ni}) = 0
$
حذف می‌شوند. 
\\
به دلیل استقلال $\epsilon_{ni}$ها داریم:
$$
\mathbb{E}[(\Sigma_{i = 1}^{D}w_i\epsilon_{ni})^2] = \Sigma_{i = 1}^{D}w_i^2\sigma^2
$$

$$
\rightarrow \mathbb{E}[E^{noisy}] = E_D + \frac{1}{2} \Sigma_{i = 1}^{D} w_i^2\sigma^2
$$